template-coq/theories/TemplateMonad/Core.v
@@ -1,7 +1,7 @@
 From Coq Require Import Strings.String.
 Open Scope string_scope.
 From MetaCoq.Template Require Import
-     Ast uGraph AstUtils Common.
+     Ast AstUtils Common.
 
 Set Universe Polymorphism.
 Set Universe Minimization ToSet.
@@ -46,7 +46,7 @@ Cumulative Inductive TemplateMonad@{t u} : Type@{t} -> Prop :=
 | tmQuoteRec : forall {A:Type@{t}}, A  -> TemplateMonad program
 (* Quote the body of a definition or inductive. Its name need not be fully qualified *)
 | tmQuoteInductive : qualid -> TemplateMonad mutual_inductive_body
-| tmQuoteUniverses : TemplateMonad uGraph.t
+| tmQuoteUniverses : TemplateMonad constraints
 | tmQuoteConstant : qualid -> bool (* bypass opacity? *) -> TemplateMonad constant_entry
 (* unquote before making the definition *)
 (* FIXME take an optional universe context as well *)
