test-suite/TypingTests.v
@@ -31,13 +31,13 @@ Unset Printing Matching.
 Ltac typecheck := try red; cbn; intros;
   match goal with
     |- ?Σ ;;; ?Γ |- ?t : ?T =>
-    eapply (infer_correct Σ Γ t T); [constructor|vm_compute; reflexivity]
+    refine (infer_correct Σ _ _ Γ t T _ _); [reflexivity|constructor|vm_compute; reflexivity]
   end.
 Ltac infer := try red;
   match goal with
     |- ?Σ ;;; ?Γ |- ?t : ?T =>
-    eapply (infer_correct Σ Γ t T); [constructor|
-      let t' := eval vm_compute in (infer Σ Γ t) in
+    refine (infer_correct Σ _ _ Γ t T _ _); [reflexivity|constructor|
+      let t' := eval vm_compute in (infer' Σ Γ t) in
           change (t' = Checked T); reflexivity]
   end.
 
@@ -47,7 +47,7 @@ Definition type_program (p : global_declarations * term) (ty : term) :=
   let Σ := reconstruct_global_context (fst p) in
   Σ ;;; [] |- snd p : ty.
 
-Example typecheck_four : type_program four natr := ltac:(typecheck).
+Example typecheck_four : type_program four natr:= ltac:(typecheck).
 
 Goal { ty & type_program four ty }.
 Proof.
@@ -159,11 +159,11 @@ Definition f2 := (forall (A:Type@{i}) (B: Prop), A -> B -> B).
 
 Quote Definition f1' := (forall (A:Type@{i}) (B: Prop), A -> B -> A). 
 
-Eval lazy in infer (nil, ConstraintSet.empty) nil f1'.
+Eval lazy in infer' (nil, ConstraintSet.empty) nil f1'.
 
 Quote Definition f2' := (forall (A:Type@{i}) (B: Prop), A -> B -> B). 
 
-Eval lazy in infer (nil, ConstraintSet.empty) nil f2'.
+Eval lazy in infer' (nil, ConstraintSet.empty) nil f2'.
 
 Definition f := (forall (A:Type@{i}) (B: Type@{j}), A -> B -> A).
 (* : Type@{i+1, j+1} *)
@@ -172,4 +172,4 @@ Quote Definition f' := (forall (A:Type@{i}) (B:Type@{j}), A -> B -> A).
 
 Quote Definition f'' := (forall (B: Type@{j}), B -> B). 
 
-Eval lazy in infer (nil, ConstraintSet.empty) nil f'.
+Eval lazy in infer' (nil, ConstraintSet.empty) nil f'.
